Finished with the Alpha_conv proof

theories/L6_PCPS/alpha_conv.v
@@ -102,7 +102,7 @@ Inductive Alpha_conv :
       Alpha_conv (Eprim x p ys e) (Eprim x' p ys' e') f
 | Alpha_Efun :
     forall B B' e e' f f',
-      Disjoint _ (name_in_fundefs B') (image f (occurs_free e) :|: bound_var e) ->
+      Disjoint _ (name_in_fundefs B') (image f (occurs_free (Efun B e)) :|: bound_var (Efun B e)) ->
       construct_fundefs_injection f B B' f' ->
       Alpha_conv_fundefs B B' f' ->
       Alpha_conv e e' f' ->
@@ -119,8 +119,7 @@ with Alpha_conv_fundefs : fundefs -> fundefs -> (var -> var) -> Prop :=
       f g = g' ->
       Alpha_conv_fundefs B B' f ->
       
-      length xs = length xs' ->
-      Disjoint _ (FromList xs) (image f (occurs_free e) :|: bound_var e) ->
+      Disjoint _ (FromList xs') (image f (occurs_free e) :|: bound_var e) ->
       construct_lst_injection f xs xs' f' ->
       Alpha_conv e e' f' ->
       
@@ -301,12 +300,43 @@ Proof.
     eapply IHHinj. eapply Disjoint_Included_r; [| eassumption ].
     sets.
 Qed.
-
   
+Lemma construct_fundefs_injection_image_subset S f B B' f' :
+  construct_fundefs_injection f B B' f' ->
+  image f' (name_in_fundefs B :|: S) \subset
+  name_in_fundefs B' :|: image f (S \\ name_in_fundefs B).
+Proof.
+  intros Hinj. revert S; induction Hinj; intros S.
+  - simpl. sets.
+  - rewrite <- Union_Setminus_Included; last reflexivity; tci.
+    simpl.
+    eapply Included_trans.
+    eapply image_extend_Included'.
+    rewrite !Setminus_Union_distr.
+    eapply Union_Included; [| sets ].
+    rewrite Setminus_Same_set_Empty_set, Union_Empty_set_neut_l. 
+    rewrite <- !Setminus_Union_distr.
+    eapply Included_trans.
+    eapply image_monotonic. eapply Setminus_Included.
+    eapply Included_trans.
+    eapply IHHinj. sets.
+Qed.
+
+Lemma construct_fundefs_injection_image_subset' f B B' f' :
+  construct_fundefs_injection f B B' f' ->
+  image f' (name_in_fundefs B) \subset name_in_fundefs B'.
+Proof.
+  intros Hinj.
+  rewrite <- (Union_Empty_set_neut_r (name_in_fundefs B)).
+  eapply Included_trans. eapply construct_fundefs_injection_image_subset.
+  eassumption. 
+  rewrite Setminus_Empty_set_abs_r, image_Empty_set. sets.
+Qed.
+
 Lemma construct_fundefs_injection_injective_pres S f B1 B2 f' :
   construct_fundefs_injection f B1 B2 f' ->
   injective_subdomain (S \\ name_in_fundefs B1) f ->
-  Disjoint _ (image f' (name_in_fundefs B1)) (image f (S \\ name_in_fundefs B1)) ->  
+  Disjoint _ (name_in_fundefs B2) (image f (S \\ name_in_fundefs B1)) ->  
   injective_subdomain (name_in_fundefs B1 :|: S) f'.
 Proof.
   intros H1 Hinj Hdis.
@@ -321,10 +351,12 @@ Proof.
   eapply f_eq_subdomain_antimon;
     [| eapply construct_fundefs_injection_f_eq_subdomain; eauto ].
   reflexivity. now sets.
-  eapply Disjoint_Included_r; [| eassumption ].
+  eapply Disjoint_Included; [| | eassumption ].
   rewrite image_f_eq_subdomain. reflexivity.
   symmetry. eapply construct_fundefs_injection_f_eq_subdomain.
   eassumption. sets.
+
+  eapply construct_fundefs_injection_image_subset'; eauto. 
 Qed.
 
 
@@ -373,7 +405,18 @@ Proof.
     eapply Included_trans.
     eapply IHHinj. sets.
 Qed.
-  
+
+Lemma construct_lst_injection_image_subset' f xs ys f' :
+  construct_lst_injection f xs ys f' ->
+  image f' (FromList xs) \subset FromList ys.
+Proof.
+  intros Hinj.
+  rewrite <- (Union_Empty_set_neut_r (FromList xs)).
+  eapply Included_trans. eapply construct_lst_injection_image_subset.
+  eassumption. 
+  rewrite Setminus_Empty_set_abs_r, image_Empty_set. sets.
+Qed.
+
 Lemma construct_lst_injection_injective_pres  S f xs ys f' :
   construct_lst_injection f xs ys f' ->
   injective_subdomain (S \\ FromList xs) f ->
@@ -391,39 +434,339 @@ Proof.
   eapply f_eq_subdomain_antimon;
     [| eapply construct_lst_injection_f_eq_subdomain; eauto ].
   reflexivity. now sets.
-  eapply injective_subdomain_Union_not_In_image; sets.
-  eapply injective_subdomain_Union. 
-  
-  eapply construct_lst_injection_injective_pres. 
+   
+  eapply Disjoint_Included_l.
+  eapply construct_lst_injection_image_subset'. eassumption.
   eapply Disjoint_Included_r; [| eassumption ].
   rewrite image_f_eq_subdomain. reflexivity.
   symmetry. eapply construct_lst_injection_f_eq_subdomain.
   eassumption. sets.
 Qed.
 
+(* TODO move *)
+Lemma image_Setminus {A B} (g : A -> B) S1 S2:
+  injective_subdomain (S1 :|: S2) g ->
+  image g (S1 \\ S2) <--> image g S1 \\ image g S2.
+Proof.
+  intros Hinj. split.
+  - intros z [z' [Hin Heq]]. inv Hin.
+    constructor.
+    now eapply In_image; eauto.
+    intros [y' [Hin' Heq']].
+    assert (Heq : y' = z').
+    { eapply Hinj; eauto. }
+    subst; contradiction.
+  - intros z [[z' [Hin Heq]] H2]. subst.
+    eapply In_image. constructor; eauto.
+    intros Hc. eapply H2. eapply In_image. eassumption.
+Qed.
 
+Lemma image_extend_injective_subdomain { A } g x (y : A) S:
+  injective_subdomain (x |: S) (g {x ~> y}) ->
+  image g (S \\ [set x]) <--> image (g {x ~> y}) S \\ [set y].
+Proof.
+  intros Hinj. split.
+  - intros z [z' [Hin Heq]]. inv Hin.
+    constructor.
+    eexists. split. eassumption.
+    rewrite extend_gso. reflexivity.
+    now intros Hc; subst; eapply H0; eauto.
+    
+    intros Hc. inv Hc.
+    assert (Heq : x = z').
+    { eapply Hinj; eauto.
+      rewrite extend_gss. rewrite extend_gso; eauto.
+      now intros Hc; subst; eapply H0; eauto. }
+    subst. eapply H0; reflexivity.
+  - intros z [[z' [Hin Heq]] H2]. subst.
+    destruct (peq x z').
+    + subst. rewrite extend_gss in H2.
+      exfalso; eauto.
+    + rewrite extend_gso; eauto.
+      eapply In_image. constructor; eauto.
+      intros Hc; inv Hc; eauto.
+Qed.
+
+
+Lemma construct_fundefs_injection_image_eq S g B1 B2 g':
+  construct_fundefs_injection g B1 B2 g' -> 
+  injective_subdomain (S \\ name_in_fundefs B1) g ->
+  Disjoint _ (name_in_fundefs B2) (image g (S \\ name_in_fundefs B1)) ->
+  image g (S \\ name_in_fundefs B1) <--> image g' S \\ name_in_fundefs B2.
+Proof.
+  intros Hc. revert S. induction Hc; intros S Hinj Hdis.
+  - simpl. rewrite !Setminus_Empty_set_neut_r. reflexivity.
+  - simpl.
+    rewrite <- !Setminus_Union.
+    rewrite <- image_extend_injective_subdomain with (y := g2).
+    + rewrite IHHc. reflexivity.
+      eapply injective_subdomain_antimon. eassumption.
+      simpl. sets.
+      eapply Disjoint_Included; [ | | eassumption ].
+      xsets. sets.
+    + eapply injective_subdomain_antimon.
+      eapply construct_fundefs_injection_injective_pres
+        with (B1 := Fcons g1 t1 xs1 e1 B1).
+      now econstructor 2; eauto.
+      eapply injective_subdomain_antimon. eassumption. sets.
+      eapply Disjoint_Included_r; last eassumption.
+      xsets.
+      rewrite Union_Setminus_Included; sets. tci.
+Qed.
+
+Lemma construct_lst_injection_image_eq S g l1 l2 g':
+  construct_lst_injection g l1 l2 g' -> 
+  injective_subdomain (S \\ FromList l1) g ->
+  Disjoint _ (FromList l2) (image g (S \\ FromList l1)) ->
+  image g (S \\ FromList l1) <--> image g' S \\ FromList l2.
+Proof.
+  intros Hc. revert S. induction Hc; intros S Hinj Hdis.
+  - simpl. normalize_sets. rewrite !Setminus_Empty_set_neut_r. reflexivity.
+  - simpl. repeat normalize_sets. 
+    rewrite <- !Setminus_Union.
+    rewrite <- image_extend_injective_subdomain with (y0 := y).
+    + rewrite IHHc. reflexivity.
+      eapply injective_subdomain_antimon. eassumption.
+      simpl. sets.
+      eapply Disjoint_Included; [ | | eassumption ].
+      xsets. sets.
+    + eapply injective_subdomain_antimon.
+      eapply construct_lst_injection_injective_pres with (xs := x :: xs).
+      econstructor 2; eauto. normalize_sets. eassumption.
+      eapply injective_subdomain_antimon. eassumption. sets.
+      normalize_sets. eapply Disjoint_Included_r; last eassumption.
+      xsets.
+      normalize_sets. 
+      rewrite Union_Setminus_Included; sets. tci.
+Qed.
+
+Lemma Forall2_map {A B} (g : A -> B) l1 l2 :
+  Forall2 (fun y y' => g y = y') l1 l2 ->
+  l2 = map g l1.
+Proof.
+  intros Hall; induction Hall; subst; eauto.
+Qed.
+
+Lemma Alpha_conv_fundefs_image_eq B B' f :
+  Alpha_conv_fundefs B B' f ->
+  image f (name_in_fundefs B) <--> name_in_fundefs B'.
+Proof.
+  intros Ha. induction Ha.
+  + rewrite image_Empty_set. reflexivity.
+  + simpl. rewrite image_Union, image_Singleton.
+    subst. rewrite IHHa. reflexivity.
+Qed.
+  
+
+Lemma Alpha_conv_occurs_free_mut :
+  (forall e e' f,
+      Alpha_conv e e' f ->
+      injective_subdomain (occurs_free e) f ->
+      image f (occurs_free e) <--> occurs_free e') /\
+  (forall B B' f,
+      Alpha_conv_fundefs B B' f ->
+      injective_subdomain (name_in_fundefs B :|: occurs_free_fundefs B) f ->
+      image f (occurs_free_fundefs B ) <-->
+      (occurs_free_fundefs B')).
+Proof with now sets.
+  exp_defs_induction IHe IHl IHB; try (intros tm g Ha Hinj; inv Ha);
+    repeat normalize_occurs_free.
+  - rewrite image_Union.
+    assert (Hinj' : injective_subdomain (v |: occurs_free e) (g {v ~> x'})).
+    { eapply injective_subdomain_extend'.
+      - rewrite Setminus_Union_distr.
+        rewrite Setminus_Same_set_Empty_set, Union_Empty_set_neut_l.  
+        eapply injective_subdomain_antimon. eassumption.
+        normalize_occurs_free...
+      - intros Hc. eapply H6. left. eapply image_monotonic; [| eassumption ]. 
+        sets. }
+    eapply Same_set_Union_compat.
+    + eapply Forall2_map in H5. subst.
+      rewrite FromList_map_image_FromList. reflexivity.
+    + eapply IHe in H7.
+      * rewrite <- H7.
+        eapply image_extend_injective_subdomain.
+        eassumption.
+      * eapply injective_subdomain_antimon; eauto...
+  - inv H1. normalize_occurs_free. rewrite image_Singleton.
+    reflexivity.
+  - destruct pats' as [| [c' e'] l']; inv H1. destruct H3 as [Heq Ha]. 
+    simpl in *; subst.
+    normalize_occurs_free. rewrite !image_Union.
+    rewrite IHe, IHl; eauto. rewrite image_Singleton. reflexivity.
+    constructor. eauto. reflexivity.
+    eapply injective_subdomain_antimon. eassumption. normalize_occurs_free...
+    eapply injective_subdomain_antimon. eassumption. normalize_occurs_free...
+  - rewrite image_Union.
+    assert (Hinj' : injective_subdomain (v |: occurs_free e) (g {v ~> x'})).
+    { eapply injective_subdomain_extend'.
+      - rewrite Setminus_Union_distr.
+        rewrite Setminus_Same_set_Empty_set, Union_Empty_set_neut_l.  
+        eapply injective_subdomain_antimon. eassumption.
+        normalize_occurs_free...
+      - intros Hc. eapply H7. left. eapply image_monotonic; [| eassumption ]. 
+        sets. }
+    eapply Same_set_Union_compat.
+    + rewrite image_Singleton. reflexivity.
+    + eapply IHe in H8.
+      * rewrite <- H8.
+        eapply image_extend_injective_subdomain.
+        eassumption.
+      * eapply injective_subdomain_antimon; eauto...
+  - rewrite !image_Union.
+    assert (Hinj' : injective_subdomain (x |: occurs_free e) (g {x ~> x'})).
+    { eapply injective_subdomain_extend'.
+      - rewrite Setminus_Union_distr.
+        rewrite Setminus_Same_set_Empty_set, Union_Empty_set_neut_l.  
+        eapply injective_subdomain_antimon. eassumption.
+        normalize_occurs_free...
+      - intros Hc. eapply H8. left. eapply image_monotonic; [| eassumption ]. 
+        sets. }
+    eapply Same_set_Union_compat.
+    + rewrite image_Singleton.
+      eapply Forall2_map in H6. subst.
+      rewrite FromList_map_image_FromList. reflexivity.
+    + eapply IHe in H9.
+      * rewrite <- H9.
+        eapply image_extend_injective_subdomain.
+        eassumption.
+      * eapply injective_subdomain_antimon; eauto...
+  - rewrite image_Union. 
+    assert (Hinj' : injective_subdomain (name_in_fundefs f2 :|: occurs_free (Efun f2 e)) f').
+    { eapply construct_fundefs_injection_injective_pres; eauto.
+      - eapply injective_subdomain_antimon; eauto. sets.
+      - eapply Disjoint_Included_r; [| eassumption ]. sets. }
+    eapply Same_set_Union_compat.
+    + rewrite image_f_eq_subdomain.
+      2:{ eapply construct_fundefs_injection_f_eq_subdomain. eassumption.
+          eapply Disjoint_sym. eapply occurs_free_fundefs_name_in_fundefs_Disjoint. }
+      rewrite IHB; eauto.  reflexivity.  
+      eapply injective_subdomain_antimon. eassumption.
+      normalize_occurs_free...
+    + rewrite construct_fundefs_injection_image_eq; eauto.
+      * rewrite IHe.
+        reflexivity.
+        eassumption.  
+        eapply injective_subdomain_antimon. eassumption. normalize_occurs_free.        
+        now rewrite !Union_assoc, Union_Setminus_Included; sets; tci.
+      * eapply injective_subdomain_antimon. eassumption. normalize_occurs_free...
+      * eapply Disjoint_Included_r; last eassumption. 
+        normalize_occurs_free. sets.
+  - rewrite !image_Union. rewrite image_Singleton.
+    eapply Forall2_map in H4. subst.
+    rewrite FromList_map_image_FromList. reflexivity.
+  - rewrite !image_Union.
+    assert (Hinj' : injective_subdomain (v |: occurs_free e) (g {v ~> x'})).
+    { eapply injective_subdomain_extend'.
+      - rewrite Setminus_Union_distr.
+        rewrite Setminus_Same_set_Empty_set, Union_Empty_set_neut_l.  
+        eapply injective_subdomain_antimon. eassumption.
+        normalize_occurs_free...
+      - intros Hc. eapply H6. left. eapply image_monotonic; [| eassumption ]. 
+        sets. }
+    eapply Same_set_Union_compat.
+    + eapply Forall2_map in H5. subst.
+      rewrite FromList_map_image_FromList. reflexivity.
+    + eapply IHe in H7.
+      * rewrite <- H7.
+        eapply image_extend_injective_subdomain.
+        eassumption.
+      * eapply injective_subdomain_antimon; eauto...
+  - rewrite image_Singleton...
+  - rewrite !image_Union.
+    rewrite Union_assoc. rewrite (Union_commut [set v]), <- Union_assoc.    
+    rewrite (Union_assoc [set g v]). rewrite (Union_commut [set (g v)]), <- Union_assoc.
+    rewrite <- Setminus_Union.
+    assert (Hsub_aux : occurs_free e \\ FromList l \subset
+                                   v |: name_in_fundefs f5 :|: (occurs_free e \\ (v |: (FromList l :|: name_in_fundefs f5)))).
+    { rewrite !Union_assoc.
+      rewrite (Union_commut [set v] (FromList l)). rewrite <- (Union_assoc (FromList l)).
+      rewrite <- Setminus_Union. rewrite Union_Setminus_Included; tci; sets. }
+        
+    rewrite image_Setminus.
+    + rewrite image_f_eq_subdomain at 1.
+      2:{ eapply construct_lst_injection_f_eq_subdomain. eassumption. sets. }
+      rewrite <- Setminus_Union. eapply Same_set_Union_compat.
+      * eapply Same_set_Setminus_compat.
+        ++ rewrite image_f_eq_subdomain at 1.
+           2:{ symmetry. eapply construct_lst_injection_f_eq_subdomain. eassumption. sets. }
+           rewrite construct_lst_injection_image_eq; [| eassumption | |]. 
+           rewrite IHe; [| eassumption |].
+           ** reflexivity.
+           ** eapply injective_subdomain_antimon; [| eapply Included_Union_r ].
+              eapply construct_lst_injection_injective_pres.
+              eassumption.
+              eapply injective_subdomain_antimon. eassumption.
+              normalize_occurs_free.
+              simpl. eapply Included_trans. eassumption. sets.
+              eapply Disjoint_Included_r; [| eassumption ]. sets.
+           ** eapply injective_subdomain_antimon. eassumption.
+              normalize_occurs_free.
+              eapply Included_trans. eassumption. sets.
+           ** eapply Disjoint_Included_r; [| eassumption ]. sets.
+        ++ assert (Heq : v |: name_in_fundefs f5 = name_in_fundefs (Fcons v t l e f5)) by reflexivity .
+           rewrite Heq, Alpha_conv_fundefs_image_eq; [| now econstructor; eauto ]. 
+           reflexivity.
+      * rewrite image_Setminus, image_Singleton.
+        rewrite IHB. reflexivity. eassumption.
+        eapply injective_subdomain_antimon. eassumption.
+        normalize_occurs_free. rewrite !Union_assoc. rewrite Union_Setminus_Included; tci; sets.
+        eapply injective_subdomain_antimon. eassumption.
+        normalize_occurs_free. rewrite !Union_assoc. rewrite Union_Setminus_Included; tci; sets.
+    + eapply injective_subdomain_antimon. eassumption.
+      eapply Union_Included; sets. 
+      simpl. normalize_occurs_free. eapply Included_trans. eassumption. sets.
+  - rewrite image_Empty_set. sets.
+Qed. 
+
+Lemma Alpha_conv_occurs_free :
+  forall e e' f,
+    Alpha_conv e e' f ->
+    injective_subdomain (occurs_free e) f ->
+    image f (occurs_free e) <--> occurs_free e'.
+Proof.
+  eapply Alpha_conv_occurs_free_mut.
+Qed.
+
+
+Lemma Alpha_conv_occurs_free_fundefs : 
+  forall B B' f,
+      Alpha_conv_fundefs B B' f ->
+      injective_subdomain (name_in_fundefs B :|: occurs_free_fundefs B) f ->
+      image f (occurs_free_fundefs B ) <--> (occurs_free_fundefs B').
+Proof.
+  eapply Alpha_conv_occurs_free_mut.
+Qed.
 
 Section Alpha_conv_correct.
 
   Variable pr : prims.
   Variable cenv : ctor_env.
-  Variable PT : Post.
+  Variable P : Post.
   Variable PG : PostG.
+  Variable (Hcompat : post_compat P P)
+           (Happcompat : post_app_compat PG P)
+           (Hletappcompat : post_letapp_compat PG P P)
+           (Hrefl : post_refl P)
+           (Hlocalstrong : (* local implies global *)
+              forall (m : nat) (e1 e2 : exp) (rho rho' : env) (c1 c2 : nat),
+                P c1 c2 -> PG m (e1, rho, c1) (e2, rho', c2))
+           (* This means that we don't support lower bound yet *)
+           (Hadd_src : forall c1 c2 c, P c1 c2 -> P (c1 + c) c2). 
 
 
   (** ** Environment relation up to renaming *)
   (* TODO move to log rel *)
 
-  Definition preord_env_P_inj (P : Ensemble var) k f rho1 rho2 :=
-    forall x : var,
-      P x -> preord_var_env pr cenv k PG rho1 rho2 x (f x).
+  Definition preord_env_P_inj (S : Ensemble var) k f rho1 rho2 :=
+    forall x : var, S x -> preord_var_env pr cenv k PG rho1 rho2 x (f x).
 
-  Lemma preord_env_P_inj_set (P : Ensemble var) (rho1 rho2 : env) 
+  Lemma preord_env_P_inj_set (S : Ensemble var) (rho1 rho2 : env) 
         (k : nat) f (x y : var) (v1 v2 : val) : 
-    preord_env_P_inj  (P \\ [set x]) k f rho1 rho2 ->
+    preord_env_P_inj  (S \\ [set x]) k f rho1 rho2 ->
     preord_val pr cenv k PG v1 v2 ->
-    injective_subdomain (x |: P) (f {x ~> y}) ->
-    preord_env_P_inj P k (f {x ~> y}) (M.set x v1 rho1) (M.set y v2 rho2).
+    injective_subdomain (x |: S) (f {x ~> y}) ->
+    preord_env_P_inj S k (f {x ~> y}) (M.set x v1 rho1) (M.set y v2 rho2).
   Proof.
     intros Henv Hv Hinj z HP. unfold extend. 
     destruct (peq z x) as [| Hneq].
@@ -440,12 +783,12 @@ Section Alpha_conv_correct.
         eexists. rewrite M.gso; eauto. 
   Qed.
   
-  Lemma preord_env_P_inj_set_alt (P : Ensemble var) (rho1 rho2 : env) 
+  Lemma preord_env_P_inj_set_alt (S : Ensemble var) (rho1 rho2 : env) 
         (k : nat) f (x y : var) (v1 v2 : val) : 
-    preord_env_P_inj (P \\ [set x]) k f rho1 rho2 ->
+    preord_env_P_inj (S \\ [set x]) k f rho1 rho2 ->
     preord_val pr cenv k PG v1 v2 ->
-    ~ In _ (image f (P \\ [set x])) y ->
-    preord_env_P_inj P k (f {x ~> y}) (M.set x v1 rho1) (M.set y v2 rho2).
+    ~ In _ (image f (S \\ [set x])) y ->
+    preord_env_P_inj S k (f {x ~> y}) (M.set x v1 rho1) (M.set y v2 rho2).
   Proof.
     intros Henv Hv Hnin z HP. unfold extend. 
     destruct (peq z x) as [| Hneq].
@@ -469,10 +812,10 @@ Section Alpha_conv_correct.
     intros Henv Hi x HP. eapply Henv. now apply Hi.
   Qed.
 
-  Lemma preord_env_P_inj_monotonic P (k j : nat) (rho1 rho2 : env) f : 
+  Lemma preord_env_P_inj_monotonic S (k j : nat) (rho1 rho2 : env) f : 
     j <= k ->
-    preord_env_P_inj P k f rho1 rho2 ->
-    preord_env_P_inj P j f rho1 rho2.
+    preord_env_P_inj S k f rho1 rho2 ->
+    preord_env_P_inj S j f rho1 rho2.
   Proof.
     intros Hleq Hpre x HP v Hget.
     edestruct Hpre as [v2 [Heq Hpre2] ]; eauto.
@@ -493,7 +836,8 @@ Section Alpha_conv_correct.
     find_def g B1 = Some (t, xs1, e1) ->
     exists xs2 e2 f', 
       find_def (f g) B2 = Some (t, xs2, e2) /\
-      construct_lst_injection f xs1 xs2 f' /\ 
+      construct_lst_injection f xs1 xs2 f' /\
+      Disjoint _ (FromList xs2) (image f (occurs_free e1) :|: bound_var e1) /\
       Alpha_conv e1 e2 f'.
   Proof.
     intros Ha Hinj Hdef. induction Ha. 
@@ -530,27 +874,8 @@ Section Alpha_conv_correct.
       edestruct IHxs as [vs2' Hset2]; try eassumption.
       eexists. simpl; rewrite Hset2; eauto.
   Qed.
-
-
-  (* Lemma extend_lst_codom  (A : Type) (f : positive -> A) (l : list positive) *)
-  (*       (l' : list A) (x : positive) : *)
-  (*   List.In (f <{ l ~> l' }> x) l' -> *)
-  (*   List.length l = List.length l' -> *)
-  (*   injective_subdomain (FromList l) (f <{ l ~> l' }>) -> *)
-  (*   List.In x l. *)
-  (* Proof. *)
-  (*   revert l'; induction l; intros l' Hin Heq Hinj; simpl in *. *)
-  (*   - destruct l'; try contradiction. inv Heq. *)
-  (*   - destruct l'; try contradiction. inv Heq. *)
-  (*     destruct (peq a x); subst; eauto. *)
-  (*     rewrite extend_gso in Hin; eauto. *)
-  (*     inv Hin.  *)
-  (*     exfalso. eapply n. eapply Hinj. left. reflexivity. *)
-  (*     right. eapply IHl. *)
-  (*     eassumption. *)
-      
-
-  Lemma preord_env_P_inj_setlist (P1 : var -> Prop) (rho1 rho2 rho1' rho2' : env)
+  
+  Lemma preord_env_P_inj_set_lists (P1 : var -> Prop) (rho1 rho2 rho1' rho2' : env)
         (k : nat) (xs1 xs2 : list var) (vs1 vs2 : list val) f f':
     preord_env_P_inj (Setminus _ P1 (FromList xs1)) k f rho1 rho2 ->
     Forall2 (preord_val pr cenv k PG) vs1 vs2 ->
@@ -564,12 +889,16 @@ Section Alpha_conv_correct.
 
     preord_env_P_inj P1 k f' rho1' rho2'.
   Proof.
-    revert P1 rho1 rho2 rho1' rho2' xs2 vs1 vs2 f f'. induction xs1;
-      intros P1 rho1 rho2 rho1' rho2' xs2 vs1 vs2  f f' Hpre Hall Hinjf Hinj Hset1 Hset2 x HP v Hget.
-    - inv Hinj. destruct vs1; try discriminate.
-      inv Hall. inv Hset1; inv Hset2. eapply Hpre; eauto.
-      constructor; eauto.
-    - destruct vs1; try discriminate. inv Hall. assert (Hinj' := Hinj). inv Hinj.
+    revert P1 rho1 rho2 rho1' rho2' xs2 vs1 vs2 f f'.
+    induction xs1;
+      intros P1 rho1 rho2 rho1' rho2' xs2 vs1 vs2  f f'
+             Hpre Hall Hinj Hdis Hlst Hset1 Hset2 x HP v Hget.
+    - inv Hlst. destruct vs1; try discriminate.
+      simpl in Hset1. inv Hset1.
+      destruct vs2; try discriminate.
+      simpl in Hset2. inv Hset2.
+      eapply Hpre; eauto. constructor; eauto.
+    - destruct vs1; try discriminate. inv Hall. assert (Hlst' := Hlst). inv Hlst.
       simpl in Hset1, Hset2. 
       destruct (set_lists xs1 vs1 rho1) eqn:Heq1;
         destruct (set_lists ys l' rho2) eqn:Heq2; try discriminate.
@@ -578,37 +907,27 @@ Section Alpha_conv_correct.
       + inv Hget. eexists. 
         simpl. unfold extend. rewrite peq_true.
         rewrite M.gss. eauto.
-      + edestruct IHxs1 with (P1 := Setminus var P1 (Singleton _ a)) as [v2 [Het' Hpre']]; eauto.
+      + edestruct IHxs1 with (P1 := Setminus var P1 (Singleton _ a)) as [v2 [Het' Hpre']];
+          eauto.
         * rewrite Setminus_Union.
           rewrite FromList_cons in Hpre. eassumption.
         * eapply injective_subdomain_antimon. eassumption. normalize_sets. sets. 
-        * constructor; eauto. intros Hc.  inv Hc; eauto.
+        * eapply Disjoint_Included; [| | eapply Hdis ].
+          normalize_sets. xsets.
+          normalize_sets. xsets.
+        * constructor; eauto. intros Hc; inv Hc; congruence.          
         * eexists. rewrite extend_gso; eauto. split; eauto.
           rewrite M.gso; [ now eauto |].
           
           intros Heq. eapply n.
           
-          eapply construct_lst_injection_injective_pres with (S := P1) in Hinj'; eauto.
-          eapply Hinj'; eauto.
+          eapply construct_lst_injection_injective_pres with (S := P1) in Hlst'; eauto.
+          eapply Hlst'; eauto.
           normalize_sets. sets.
           rewrite extend_gss.
           rewrite extend_gso. eassumption. eassumption.
-
-          
-          eapply Disjoint_Included_r.
-          rewrite image_f_eq_subdomain. reflexivity.
-          eapply construct_lst_injection_f_eq_subdomain.
-          eapply Hinj'. sets.
-          
-          eapply injective_subdomain_Union_not_In_image; [| sets ].
-          
-          eapply construct_lst_injection_injective_pres. eassumption.
-          eapply injective_subdomain_antimon. eassumption. sets.
-          
-          eassumption. eapply H7; try now constructor.
-          rewrite extend_gss. rewrite extend_gso; eassumption. 
   Qed.
-
+  
   
   Lemma preord_env_P_inj_set_lists_alt (P1 : var -> Prop) (rho1 rho2 rho1' rho2' : env)
         (k : nat) (xs1 xs2 : list var) (vs1 vs2 : list val) f :
@@ -663,9 +982,9 @@ Section Alpha_conv_correct.
           eauto.
   Qed.
 
-  Lemma Forall2_preord_var_env_map k P σ rho rho' l :
-    preord_env_P_inj P k σ rho rho' ->
-    Included _ (FromList l) P ->
+  Lemma Forall2_preord_var_env_map k S σ rho rho' l :
+    preord_env_P_inj S k σ rho rho' ->
+    Included _ (FromList l) S ->
     Forall2 (preord_var_env pr cenv k PG rho rho') l (map σ l).
   Proof with now eauto with Ensembles_DB.
     induction l; intros Henv Hin; simpl; constructor.
@@ -675,9 +994,9 @@ Section Alpha_conv_correct.
       rewrite FromList_cons...
   Qed.
 
-  Lemma preord_env_P_inj_get_list_l (P : var -> Prop) k f rho1 rho2 xs vs1 :
-    preord_env_P_inj P k f rho1 rho2 ->
-    Included var (FromList xs) P ->
+  Lemma preord_env_P_inj_get_list_l (S : var -> Prop) k f rho1 rho2 xs vs1 :
+    preord_env_P_inj S k f rho1 rho2 ->
+    Included var (FromList xs) S ->
     get_list xs rho1 = Some vs1 ->
     exists vs2 : list val,
       get_list (map f xs) rho2 = Some vs2 /\ Forall2 (preord_val pr cenv k PG) vs1 vs2.
@@ -688,7 +1007,8 @@ Section Alpha_conv_correct.
       destruct (M.get a rho1) eqn:Hgeta; try discriminate.
       destruct (get_list xs rho1) eqn:Hgetl; try discriminate.
       inv Hget.
-      edestruct Henv with (x := a) as [x' [Hgetx' Hprex']]. eapply Hinc. rewrite FromList_cons...
+      edestruct Henv with (x := a) as [x' [Hgetx' Hprex']]. eapply Hinc.
+      rewrite FromList_cons...
       eassumption.
       edestruct IHxs as [l' [Hgetl' Hprel']]. eassumption.
       eapply Included_trans; [| eassumption ]. rewrite FromList_cons...
@@ -698,28 +1018,28 @@ Section Alpha_conv_correct.
       now constructor; eauto.
   Qed.
 
-  Global Instance preord_env_P_inj_f_proper : Proper (eq ==> eq ==> f_eq ==> eq ==> eq ==> iff)
-                                                preord_env_P_inj.
+  Global Instance preord_env_P_inj_f_proper :
+    Proper (eq ==> eq ==> f_eq ==> eq ==> eq ==> iff) preord_env_P_inj.
   Proof.
     constructor; subst; intros Hp.
     intros z Hz. rewrite <- H1. eauto.
     intros z Hz. rewrite H1. eauto.
   Qed.
 
-  Lemma preord_env_P_inj_set_not_In_P_l P k f rho1 rho2 x v :
-    preord_env_P_inj P k f rho1 rho2 ->
-    ~ In _ P x ->
-    preord_env_P_inj P k f (M.set x v rho1) rho2.
+  Lemma preord_env_P_inj_set_not_In_P_l S k f rho1 rho2 x v :
+    preord_env_P_inj S k f rho1 rho2 ->
+    ~ In _ S x ->
+    preord_env_P_inj S k f (M.set x v rho1) rho2.
   Proof.
     intros Henv Hnin y Hy v' Hget. eapply Henv. eassumption.
     rewrite M.gso in Hget. eassumption. intros Hc; subst.
     eauto.
   Qed.
 
-  Lemma preord_env_P_inj_set_not_In_P_r P k f rho1 rho2 x v :
-    preord_env_P_inj P k f rho1 rho2 ->
-    ~ In _ (image f P) x ->    
-    preord_env_P_inj P k f rho1 (M.set x v rho2).
+  Lemma preord_env_P_inj_set_not_In_P_r S k f rho1 rho2 x v :
+    preord_env_P_inj S k f rho1 rho2 ->
+    ~ In _ (image f S) x ->    
+    preord_env_P_inj S k f rho1 (M.set x v rho2).
   Proof.
     intros Henv Hnin y Hy v' Hget.
     edestruct Henv as [v'' [Hget' Hv]]; eauto.
@@ -728,11 +1048,11 @@ Section Alpha_conv_correct.
     eapply Hnin. eexists; eauto.
   Qed.
   
-  Lemma preord_env_P_inj_reset P k f rho rho' x y v :
+  Lemma preord_env_P_inj_reset S k f rho rho' x y v :
     M.get (f x) rho' = Some v ->
-    ~ In _ (image f P) y ->
-    preord_env_P_inj P k f rho rho' ->
-    preord_env_P_inj P k (f {x ~> y}) rho (M.set y v rho').
+    ~ In _ (image f S) y ->
+    preord_env_P_inj S k f rho rho' ->
+    preord_env_P_inj S k (f {x ~> y}) rho (M.set y v rho').
   Proof.
     intros Hget Hnin Hpre z Hz v' Hget'.
     destruct (peq z x); subst.
@@ -745,14 +1065,14 @@ Section Alpha_conv_correct.
       intros Hc; subst. eapply Hnin; eexists; eauto.
   Qed.
 
-  Lemma preord_env_P_inj_reset_lists P k f rho rho' rho'' xs ys vs :
+  Lemma preord_env_P_inj_reset_lists S k f rho rho' rho'' xs ys vs :
     get_list (map f xs) rho' = Some vs ->
-    Disjoint _ (image f P) (FromList ys) ->
+    Disjoint _ (image f S) (FromList ys) ->
     set_lists ys vs rho' = Some rho'' ->
     NoDup ys ->
     length xs = length ys ->
-    preord_env_P_inj P k f rho rho' ->
-    preord_env_P_inj P k (f <{xs ~> ys}>) rho rho''.
+    preord_env_P_inj S k f rho rho' ->
+    preord_env_P_inj S k (f <{xs ~> ys}>) rho rho''.
   Proof.
     revert rho'' ys vs; induction xs; intros rho'' ys vs Hget HD Hset Hdup Hlen Hpre.
     - simpl. destruct vs; try discriminate.
@@ -764,7 +1084,7 @@ Section Alpha_conv_correct.
       destruct ys; try discriminate. simpl in Hset.
       destruct (set_lists ys l rho') eqn:Hsetl; try discriminate.
       rewrite FromList_cons in HD. inv Hset.
-      assert (Hpre' : preord_env_P_inj P k (f <{ xs ~> ys }>) rho t).
+      assert (Hpre' : preord_env_P_inj S k (f <{ xs ~> ys }>) rho t).
       { eapply IHxs. reflexivity.
         now eauto with Ensembles_DB.
         eassumption. now inv Hdup. now inv Hlen. eassumption. }
@@ -788,133 +1108,258 @@ Section Alpha_conv_correct.
         reflexivity.
   Qed.
 
-  Lemma preord_env_P_inj_def_funs_pre k rho1 rho2 B1 B1' B2 f h h' e :
+  Lemma construct_lst_injection_length f xs1 xs2 f' :
+    construct_lst_injection f xs1 xs2 f' ->
+    List.length xs1 = List.length xs2.
+  Proof.
+    intros Hinj. induction Hinj.
+    - reflexivity.
+    - simpl. congruence.
+  Qed.
+  
+  Lemma preord_env_P_inj_def_funs_pre k S rho1 rho2 B1 B2 f h :
     (* The IH *)
     (forall m : nat,
        m < k ->
        forall (e1 e2 : exp) (rho1 rho2 : env) (f : var -> var),
-         injective f ->
+         injective_subdomain (occurs_free e1) f ->
          Alpha_conv e1 e2 f ->
          preord_env_P_inj (occurs_free e1) m f rho1 rho2 ->
-         preord_exp pr cenv m PT PG (e1, rho1) (e2, rho2)) ->
+         preord_exp pr cenv m P PG (e1, rho1) (e2, rho2)) ->
     construct_fundefs_injection f B1 B2 h ->
-    injective_subdomain (occurs_free e) f ->
-    Alpha_conv_fundefs B1 B2 h'  ->
-    preord_env_P_inj (occurs_free (Efun B1' e)) k f rho1 rho2 ->
-    preord_env_P_inj (occurs_free (Efun B1' e) :|: (name_in_fundefs B1)) k h
+    Disjoint _ (image f S) (name_in_fundefs B2) ->
+    injective_subdomain S f ->
+    occurs_free_fundefs B1 \subset S ->
+    Alpha_conv_fundefs B1 B2 h  ->
+    preord_env_P_inj S k f rho1 rho2 ->
+    preord_env_P_inj (name_in_fundefs B1 :|: S) k h
                      (def_funs B1 B1 rho1 rho1) (def_funs B2 B2 rho2 rho2).
   Proof with now eauto with Ensembles_DB.
-    revert B1 rho1 rho2 B1' B2 B2' f h h' e.
+    revert S rho1 rho2 B1 B2 f h.
     induction k as [ k IH' ] using lt_wf_rec1.
-    induction B1; intros rho1 rho2 B1' B2 B2' g h h' e' IHe Hinj Hinj' Hinj'' Ha Ha' Hpre.
-    - inv Ha. simpl. subst. inv Hinj. eapply preord_env_P_inj_set. 
-      + eapply preord_env_P_inj_antimon. now eapply IHB1; eauto.
-        eauto 6 with Ensembles_DB.
-      + rewrite preord_val_eq.
-        intros vs1 vs2 j t1 xs1 e1 rho1' Hlen Hf Hs.
-        edestruct Alpha_conv_fundefs_find_def
-          as [xs2 [e2 [f'' [Hf' [Hlen' [Hinj''' Ha'' ] ] ] ] ] ]; [ apply Ha' | | | ]; eauto.
-        now eapply construct_fundefs_injection_injective; eauto.
-        edestruct set_lists_length2 as [rho2' Hs']; eauto.
-        exists xs2. exists e2. exists rho2'. split; eauto.
-        admit.
-        (*split; [ now eauto |]. intros Hleq Hpre'.
-        eapply IHe; [| | eassumption |]. omega.
-        eapply construct_lst_injection_injective; eauto.
-        now eapply construct_fundefs_injection_injective; eauto.
-        apply find_def_correct in Hf; eauto.
-        eapply preord_env_P_inj_antimon; [| eapply occurs_free_in_fun; eassumption ]. 
-        * eapply preord_env_P_inj_set_lists;
-          [ | eassumption | eassumption | now eauto | now eauto  ].
-          eapply preord_env_P_inj_antimon.
-          eapply IH'; eauto. intros. eapply IHe. omega. now eauto. now eauto.
-          eassumption.
-          eapply (preord_env_P_inj_monotonic _ k). omega.
-          now eauto. rewrite Setminus_Union_distr.
-          rewrite Setminus_Same_set_Empty_set.
-          normalize_occurs_free... *)
-      + eapply injective_subdomain_antimon. eassumption.
-        constructor.
-    - inv Ha. simpl. inv Hinj. eapply preord_env_P_inj_antimon. eassumption.
-      eauto with Ensembles_DB.
-  Admitted.
+    intros S rho1 rho2 B1 B2 f h IHe Hlst Hdis Hinj Hsub Ha Hpre.
+    - intros x Hin v Hget.
+      destruct (Decidable_name_in_fundefs B1) as [Dec].
+      destruct (Dec x).
+      + rewrite def_funs_eq in Hget; eauto. inv Hget.
+        assert (Him : (h x) \in name_in_fundefs B2).
+        { eapply Included_trans.
+          eapply construct_fundefs_injection_image_subset'. eassumption.
+          sets. eapply In_image. eassumption. }        
+        eexists. split.
+        eapply def_funs_eq. eassumption.
 
-(*
-Needs : 1.) Fixing the right assumptions for the bounds
-        2.) Uses the updated compat lemmas (m < k)
+        { rewrite preord_val_eq.
+          intros vs1 vs2 j t1 xs1 e1 rho1' Hlen Hf Hs.
+          edestruct Alpha_conv_fundefs_find_def
+            as [xs2 [e2 [f'' [Hf' [Hinj''' [Hdis' Ha'' ] ] ] ] ] ]; eauto.
+          now eapply construct_fundefs_injection_injective; eauto.
+          assert (Hlen' := Hinj''').
+          eapply construct_lst_injection_length in Hlen'.
+          
+          edestruct set_lists_length2 as [rho2' Hs']; eauto.
+          exists xs2. exists e2. exists rho2'. split; eauto.
+          split; [ now eauto |]. intros Hleq Hpre'.
+          eapply preord_exp_post_monotonic;
+            first (intros ? ? ?; eapply Hlocalstrong; eassumption).
+          
+          assert (Hinjh : injective_subdomain (occurs_free e1 \\ FromList xs1) h).
+          { eapply injective_subdomain_antimon   
+              with (S0 := name_in_fundefs B1 :|: (occurs_free e1 \\ FromList xs1)); sets.
+            eapply construct_fundefs_injection_injective_pres; first eassumption.
+            * eapply injective_subdomain_antimon. eassumption.
+              do 2 eapply Setminus_Included_Included_Union.
+              eapply Included_trans.
+              eapply occurs_free_in_fun. eapply find_def_correct. eassumption.
+              sets.
+            * eapply Disjoint_sym. eapply Disjoint_Included_l; [| eassumption ].
+              eapply image_monotonic. eapply Included_trans; [| eassumption ].
+              do 2 eapply Setminus_Included_Included_Union.
+              eapply Included_trans.
+              eapply occurs_free_in_fun. eapply find_def_correct. eassumption.
+              sets. }
+          
+          eapply IHe.
+          + eassumption.
+          + eapply injective_subdomain_antimon 
+              with (S0 :=  FromList xs1 :|: occurs_free e1); sets.
+            eapply construct_lst_injection_injective_pres. eassumption.
+            eassumption. 
+            eapply Disjoint_Included_r; [| eassumption ]. sets.
+          + eassumption.
+          + eapply preord_env_P_inj_set_lists;
+              [ | eassumption | |  | now eauto | now eauto | now eauto ].
+            eapply preord_env_P_inj_antimon.
+            * eapply IH'; try eassumption.
+              ** intros. eapply IHe; eauto. omega.
+              ** eapply (preord_env_P_inj_monotonic _ k). omega.
+                 eassumption.
+            * eapply Setminus_Included_Included_Union.
+              eapply Included_trans.
+              eapply occurs_free_in_fun. eapply find_def_correct. eassumption.
+              sets.            
+            * eassumption.
+            * eapply Disjoint_Included_r; [| eassumption ].
+              sets. }
+      + inv Hin; try contradiction. setoid_rewrite def_funs_neq.
+        assert (Hfeq : h x = f x). 
+        { erewrite <- construct_fundefs_injection_f_eq_subdomain
+            with (S := S \\ name_in_fundefs B1);
+            try eassumption; sets. constructor; eauto. }
+        setoid_rewrite Hfeq. rewrite def_funs_neq in Hget; eauto.
+        eapply Hpre; eauto.
+        simpl. eapply Disjoint_In_l with (s1 := image h (S \\ name_in_fundefs B1)).
+        rewrite image_f_eq_subdomain;
+          [| symmetry; eapply construct_fundefs_injection_f_eq_subdomain; eauto ]; sets.
+        eapply In_image. constructor; eauto.
+  Qed.
 
   (** α-equivalence preserves semantics *)
   Lemma Alpha_conv_correct k rho1 rho2 e1 e2 g :
-    injective g ->
+    injective_subdomain (occurs_free e1) g ->
+    (* Disjoint _ (image g (occurs_free e1)) (bound_var e1) ->     *)
     Alpha_conv e1 e2 g ->
     preord_env_P_inj (occurs_free e1) k g rho1 rho2 ->
-    preord_exp pr cenv k PT PG (e1, rho1) (e2, rho2).
-  Proof with now eauto with Ensembles_DB. 
+    preord_exp pr cenv k P PG (e1, rho1) (e2, rho2).
+  Proof with now sets. 
     revert e1 e2 rho1 rho2 g.
     induction k as [ k IH ] using lt_wf_rec1.
-    induction e1 using exp_ind'; intros e2 rho1 rho2 g Hinj Ha Henv; inv Ha.
-    - eapply preord_exp_const_compat; eauto; intros.
-      admit.
-      + eapply Forall2_app; [ eassumption |].
-        intros x y Hin Heq. specialize (Henv x).
+    induction e1 using exp_ind'; intros e2 rho1 rho2 g Hinj (* Hdis *) Ha Henv; inv Ha.
+    - (* Econstr *)
+      eapply preord_exp_const_compat; eauto; intros.
+      + eapply Forall2_monotonic_strong; [ | eassumption ].
+        intros x y Hin1 Hin2 Heq. specialize (Henv x).
         rewrite Heq in Henv. eapply Henv.
         now constructor.
-      + eapply IHe1. eassumption. eassumption.
-        eapply preord_env_P_inj_set. 
-        eapply preord_env_P_inj_antimon; eauto.
-        normalize_occurs_free...
-        rewrite preord_val_eq. constructor; eauto using Forall2_Forall2_asym_included.
-        eapply injective_subdomain_antimon. eassumption. now constructor.
-    - inv H1. eapply preord_exp_case_nil_compat.
-    - inv H1. destruct H2 as [Heq Ha]. destruct y as [c' e2]. simpl in Heq; subst.
+      + assert (Hinj' : injective_subdomain (v |: occurs_free e1) (g {v ~> x'})).
+        { eapply injective_subdomain_extend'.
+          - rewrite Setminus_Union_distr.
+            rewrite Setminus_Same_set_Empty_set, Union_Empty_set_neut_l.  
+            eapply injective_subdomain_antimon. eassumption. normalize_occurs_free...
+          - intros Hc. eapply H6. left. eapply image_monotonic; [| eassumption ]. 
+            sets. }
+        eapply IH; try eassumption.
+        * eapply injective_subdomain_antimon; eauto...
+        * eapply preord_env_P_inj_set.
+          eapply preord_env_P_inj_antimon. eapply preord_env_P_inj_monotonic; [| eassumption ]. 
+          omega. normalize_occurs_free...
+          rewrite preord_val_eq. constructor; eauto using Forall2_Forall2_asym_included.
+          eassumption.
+    - (* Ecase nil *)
+      inv H1. eapply preord_exp_case_nil_compat.
+    - (* Ecase cons *)
+      inv H1. destruct H2 as [Heq Ha]. destruct y as [c' e2]. simpl in Heq; subst.
       eapply preord_exp_case_cons_compat; eauto.
-      admit.
-      admit.
-      eapply Forall2_monotonic; [| eassumption ]. intros x1 x2 H; now inv H. 
-      eapply IHe1. eassumption. eassumption.
-      eapply preord_env_P_inj_antimon.
-      eassumption. normalize_occurs_free...
-      eapply IHe0. eassumption. now constructor; eauto.
-      eapply preord_env_P_inj_antimon.
-      eassumption. normalize_occurs_free...
-    - eapply preord_exp_proj_compat; eauto; intros.
-      admit. 
-      eapply IHe1. eassumption. eassumption.
-      eapply preord_env_P_inj_set. 
-      eapply preord_env_P_inj_antimon; eauto.
-      normalize_occurs_free... eassumption.
-      eapply injective_subdomain_antimon. eassumption. now constructor.
-    - eapply preord_exp_fun_compat; eauto.
-      admit.
-      eapply IHe1; [| eassumption |].
-      eapply construct_fundefs_injection_injective. eassumption. eassumption.
-      eapply preord_env_P_inj_antimon.
-      + eapply preord_env_P_inj_def_funs_pre; eauto.
-      + eapply occurs_free_Efun_Included.
-    - eapply preord_exp_app_compat.
-      admit.
-      + now eauto.
-      + eapply Forall2_app; [ eassumption |].
-        intros x y Hin Heq. specialize (Henv x).
+      + eapply Forall2_monotonic; [| eassumption ]. intros x1 x2 H; now inv H.
+      + intros m Hlt. eapply IH; eauto.
+        * eapply injective_subdomain_antimon. eassumption.
+          normalize_occurs_free...
+        * eapply preord_env_P_inj_antimon. eapply preord_env_P_inj_monotonic; [| eassumption ].
+          omega. normalize_occurs_free...
+      + eapply IHe0.
+        * eapply injective_subdomain_antimon. eassumption.
+          normalize_occurs_free...
+        * now constructor; eauto.
+        * eapply preord_env_P_inj_antimon. eapply preord_env_P_inj_monotonic; [| eassumption ].
+          omega. normalize_occurs_free...
+    - (* Eproj *)
+      eapply preord_exp_proj_compat; eauto; intros.
+      assert (Hinj' : injective_subdomain (v |: occurs_free e1) (g {v ~> x'})).
+      { eapply injective_subdomain_extend'.
+        - rewrite Setminus_Union_distr.
+          rewrite Setminus_Same_set_Empty_set, Union_Empty_set_neut_l.  
+          eapply injective_subdomain_antimon. eassumption. normalize_occurs_free...
+        - intros Hc. eapply H7. left. eapply image_monotonic; [| eassumption ]. 
+          sets. }
+      eapply IH; try eassumption.
+      * eapply injective_subdomain_antimon; eauto...
+      * eapply preord_env_P_inj_set.
+        eapply preord_env_P_inj_antimon. eapply preord_env_P_inj_monotonic; [| eassumption ]. 
+        omega. normalize_occurs_free... eassumption. eassumption.    
+    - (* Eletapp *)
+      eapply preord_exp_letapp_compat; eauto; intros.
+      + eapply Henv. econstructor. now left.
+      + eapply Forall2_monotonic_strong; [ | eassumption ].
+        intros z y Hin1 Hin2 Heq. specialize (Henv z).
         rewrite Heq in Henv. eapply Henv.
-        now constructor.
+        constructor. now right.
+      + assert (Hinj' : injective_subdomain (x |: occurs_free e1) (g {x ~> x'})).
+        { eapply injective_subdomain_extend'.
+          - rewrite Setminus_Union_distr.
+            rewrite Setminus_Same_set_Empty_set, Union_Empty_set_neut_l.  
+            eapply injective_subdomain_antimon. eassumption. normalize_occurs_free...
+          - intros Hc. eapply H8. left. eapply image_monotonic; [| eassumption ]. 
+            sets. }
+        eapply IH; try eassumption.
+        * eapply injective_subdomain_antimon; eauto...
+        * eapply preord_env_P_inj_set.
+          eapply preord_env_P_inj_antimon. eapply preord_env_P_inj_monotonic; [| eassumption ]. 
+          omega. normalize_occurs_free... eassumption. eassumption.
+    - (* Efun *)
+      eapply preord_exp_fun_compat.
+      + intros.
+        assert (Heq : PS.cardinal (fundefs_fv B') =
+                      PS.cardinal (@mset (FromList (map f' (PS.elements (fundefs_fv f2)))) _)).
+        { rewrite !PS.cardinal_spec. eapply Same_set_FromList_length'.
+          eapply NoDupA_NoDup. now eapply PS.elements_spec2w.
+          eapply NoDupA_NoDup. now eapply PS.elements_spec2w.
+          rewrite <- !FromSet_elements, <- !fundefs_fv_correct, <- mset_eq.
+          rewrite FromList_map_image_FromList, <- !FromSet_elements, <- !fundefs_fv_correct.
+          rewrite Alpha_conv_occurs_free_fundefs; [ reflexivity | eassumption | ].
+          eapply construct_fundefs_injection_injective_pres. eassumption.
+          eapply injective_subdomain_antimon. eassumption. normalize_occurs_free. sets.
+          eapply Disjoint_Included_r; [| eassumption ]. normalize_occurs_free. sets. }
+        rewrite Heq.
+        rewrite PS_cardinal_map_eq.  
+        rewrite Proper_carinal. eapply Hcompat. eassumption.
+        eapply Same_set_From_set. rewrite <- mset_eq. reflexivity.
+        rewrite <- FromSet_elements, <- fundefs_fv_correct. 
+        eapply injective_subdomain_f_eq_subdomain.
+        eapply injective_subdomain_antimon. eassumption. normalize_occurs_free. sets.
+        eapply construct_fundefs_injection_f_eq_subdomain. eassumption.
+        eapply Disjoint_sym. eapply occurs_free_fundefs_name_in_fundefs_Disjoint. 
+      + eapply IHe1; [| eassumption |].
+        * eapply injective_subdomain_antimon.
+          eapply construct_fundefs_injection_injective_pres.
+          eassumption.
+          eapply injective_subdomain_antimon. eassumption.
+          normalize_occurs_free. eapply Included_Union_r. 
+          eapply Disjoint_Included_r; [| eassumption ].
+          normalize_occurs_free...
+          now sets.
+        * eapply preord_env_P_inj_antimon
+            with (P2 := name_in_fundefs f2 :|: occurs_free (Efun f2 e1)).
+          eapply preord_env_P_inj_def_funs_pre; eauto.
+          ** eapply Disjoint_sym. eapply Disjoint_Included_r;[| eassumption ]...
+          ** normalize_occurs_free...
+          ** normalize_occurs_free.
+             rewrite !Union_assoc, Union_Setminus_Included; sets. tci.
+    - eapply preord_exp_app_compat; eauto.
+      eapply Forall2_monotonic_strong; [| eassumption ]. 
+      intros x y Hin1 Hin2 Heq. specialize (Henv x).
+      rewrite Heq in Henv. eapply Henv.
+      now constructor.
     - eapply preord_exp_prim_compat; eauto; intros.
-      admit.
-      + eapply Forall2_app; [ eassumption |].
-        intros x y Hin Heq. specialize (Henv x).
+      + eapply Forall2_monotonic_strong; [| eassumption ].
+        intros x y Hin1 Hin2 Heq. specialize (Henv x).
         rewrite Heq in Henv. eapply Henv.
         now constructor.
-      + eapply IHe1. eassumption. eassumption.
-        eapply preord_env_P_inj_set. 
-        eapply preord_env_P_inj_antimon; eauto.
-        normalize_occurs_free...
-        eassumption.
-        eapply injective_subdomain_antimon. eassumption. now constructor.
-    - eapply preord_exp_halt_compat.
-      admit.
-      eapply Henv. now constructor.
-  Admitted.
-*)
+      + assert (Hinj' : injective_subdomain (v |: occurs_free e1) (g {v ~> x'})).
+        { eapply injective_subdomain_extend'.
+          - rewrite Setminus_Union_distr.
+            rewrite Setminus_Same_set_Empty_set, Union_Empty_set_neut_l.  
+            eapply injective_subdomain_antimon. eassumption. normalize_occurs_free...
+          - intros Hc. eapply H6. left. eapply image_monotonic; [| eassumption ]. 
+            sets. }
+        eapply IH; try eassumption.
+        * eapply injective_subdomain_antimon; eauto...
+        * eapply preord_env_P_inj_set.
+          eapply preord_env_P_inj_antimon. eapply preord_env_P_inj_monotonic; [| eassumption ]. 
+          omega. normalize_occurs_free...
+          eassumption. eassumption.
+    - eapply preord_exp_halt_compat; eauto.
+  Qed.
+  
 End Alpha_conv_correct.
 
 Close Scope fun_scope.
